tests/ImpBrTest/extracted/Extract.v
@@ -5,5 +5,7 @@ Require ImpBrEx.ImpBrEx.
 Extraction Language OCaml.
 Extraction Blacklist String List Char Core Z.
 
+Cd "extracted".
 Recursive Extraction Library ExtrOcamlIntConv.
 Recursive Extraction Library ImpBrEx.
+Cd "..".
